swing at proofs for semantics

src/OpalSemantics.v
@@ -1,4 +1,4 @@
-Require Import ListSet CpdtTactics FSetAVL FMapAVL OrderedType.
+Require Import CpdtTactics Orders MSetAVL FMapAVL MSets Setoid Morphisms.
 
 Set Implicit Arguments.
 
@@ -12,110 +12,84 @@ Proof.
 Qed.
 Hint Resolve eq_dec_pair.
 
-Module OrderedPair(L R: OrderedType) <: OrderedType.
-  Module LFacts := OrderedTypeFacts(L).
-  Module RFacts := OrderedTypeFacts(R).
+Module OrderedTypeOld(T: Orders.OrderedType) <: Structures.OrderedType.OrderedType.
+  Definition t := T.t.
+  Definition eq := T.eq.
+  Definition lt := T.lt.
 
-  Definition t := (L.t * R.t) % type.
-
-  Inductive eq' : t -> t -> Prop :=
-  | LeftRightEq : forall ll lr rl rr,
-      L.eq ll rl ->
-      R.eq lr rr ->
-      eq' (ll, lr) (rl, rr).
-  Definition eq := eq'.
-
-  Inductive lt' : t -> t -> Prop :=
-  | LeftLt : forall ll lr rl rr,
-      L.lt ll rl ->
-      lt' (ll, lr) (rl, rr)
-  | RightLt : forall ll lr rl rr,
-      L.eq ll rl ->
-      R.lt lr rr ->
-      lt' (ll, lr) (rl, rr).
-  Definition lt := lt'.
-
-  Theorem eq_refl : forall x, eq x x.
+  Theorem eq_refl : forall x : t, eq x x.
   Proof.
-    unfold eq.
-    specialize L.eq_refl.
-    specialize R.eq_refl.
-    intros.
-    destruct x.
-    constructor; auto.
+    specialize T.eq_equiv. crush.
   Qed.
 
-  Theorem eq_sym : forall x y, eq x y -> eq y x.
-  Proof.
-    intros. unfold eq in *. inversion H. constructor; auto.
-  Qed.
+  Theorem eq_sym : forall x y : t, eq x y -> eq y x.
+    Proof.
+      specialize T.eq_equiv. crush.
+    Qed.
 
-  Theorem eq_trans : forall x y z, eq x y -> eq y z -> eq x z.
-  Proof.
-    destruct x, y, z.
-    intros. unfold eq in *. inversion H. inversion H0.
-    specialize (L.eq_trans H4 H10).
-    specialize (R.eq_trans H6 H12).
-    constructor; auto.
-  Qed.
+  Theorem eq_trans : forall x y z : t, eq x y -> eq y z -> eq x z.
+    Proof.
+      specialize T.eq_equiv. crush.
+    Qed.
 
-  Theorem lt_trans : forall x y z, lt x y -> lt y z -> lt x z.
-    destruct x, y, z.
-    intros. unfold lt in *.
-    inversion H; inversion H0 ; subst.
-    * specialize (L.lt_trans H2 H7). intros. constructor. auto.
-    * specialize (LFacts.lt_eq H2 H9). intros. constructor. auto.
-    * specialize (LFacts.eq_lt H4 H8). intros. constructor. auto.
-    * constructor 2.
-      - specialize (L.eq_trans H4 H10). intuition.
-      - specialize (R.lt_trans H6 H12). intuition.
-  Qed.
+    Theorem lt_trans : forall x y z : t, lt x y -> lt y z -> lt x z.
+    Proof.
+      specialize T.lt_strorder.
+      intros.
+      unfold lt in *.
+      destruct H.
+      eapply StrictOrder_Transitive. apply H0. apply H1.
+    Qed.
 
-  Theorem lt_not_eq : forall x y, lt x y -> ~ eq x y.
-  Proof.
-    intros.
-    destruct x,y.
-    unfold not. intros. unfold eq in *. unfold lt in *. inversion H0.
-    inversion H; subst.
-    * specialize (L.lt_not_eq H8 H4). auto.
-    * specialize (R.lt_not_eq H12 H6). auto.
-  Qed.
+    Theorem lt_not_eq : forall x y : t, lt x y -> ~ eq x y.
+    Proof.
+      specialize T.eq_equiv.
+      specialize T.lt_strorder.
+      intros.
+      unfold lt in *.
+      destruct H, H0.
+      unfold not. intros.
+      specialize (T.lt_compat H (Equivalence_Reflexive y)).
+      crush.
+      eapply StrictOrder_Irreflexive. apply H0.
+    Qed.
 
-  Theorem compare : forall x y, Compare lt eq x y.
-  Proof.
-    destruct x, y.
-    destruct (L.compare t0 t2).
-    * constructor 1. constructor. auto.
-    * destruct (R.compare t1 t3).
-      - constructor 1. constructor 2; auto.
-      - constructor 2. constructor; auto.
-      - constructor 3. constructor 2; auto.
-    * constructor 3. constructor. auto.
-  Qed.
+    Print Module Type OrderedType.
 
-  Theorem eq_dec : forall x y, {eq x y} + {~ eq x y}.
-  Proof.
-    destruct x, y.
-    destruct (L.eq_dec t0 t2).
-    * destruct (R.eq_dec t1 t3).
-      - left. constructor; auto.
-      - right. intuition. inversion H. intuition.
-    * right. intuition. inversion H. intuition.
-  Qed.
-End OrderedPair.
+    Definition compare : forall x y : t, Structures.OrderedType.Compare lt eq x y.
+    Proof.
+      intros.
+      specialize (T.compare_spec x y).
+      destruct (T.compare x y) ; intros.
+      * constructor 2.
+        inversion H. auto.
+      * constructor 1.
+        inversion H. auto.
+      * constructor 3.
+        inversion H. auto.
+    Qed.
+
+    Definition eq_dec := T.eq_dec.
+End OrderedTypeOld.
 
 Module Opal (NodeType VarType WorldVarType OpType: OrderedType).
-  Module NodeVarType := OrderedPair(NodeType)(VarType).
+  Module NodeVarType := PairOrderedType(NodeType)(VarType).
 
-  Module NodeMap := FMapAVL.Make(NodeType).
-  Module NodeSet := FSetAVL.Make(NodeType).
-  Module VarMap := FMapAVL.Make(VarType).
-  Module NodeVarMap := FMapAVL.Make(NodeVarType).
-  Module WorldVarMap := FMapAVL.Make(WorldVarType).
-  Module OpMap := FMapAVL.Make(OpType).
+  Module NodeVarType' := OrderedTypeOld(NodeVarType).
+  Module WorldVarType' := OrderedTypeOld(WorldVarType).
+  Module OpType' := OrderedTypeOld(OpType).
+
+  Module NodeSet := MSetAVL.Make(NodeType).
+  Module NodeVarMap := FMapAVL.Make(NodeVarType').
+  Module NodeVarSet := MSetAVL.Make(NodeVarType).
+  Module NodeVarProps := MSetProperties.Properties NodeVarSet.
+  Module WorldVarMap := FMapAVL.Make(WorldVarType').
+  Module WorldVarSet := MSetAVL.Make(WorldVarType).
+  Module OpMap := FMapAVL.Make(OpType').
+  Module OpSet := MSetAVL.Make(OpType).
 
   Definition node := NodeType.t.
-  Definition var := VarMap.key.
+  Definition var := VarType.t.
   Definition worldvar := WorldVarMap.key.
   Definition op := OpMap.key.
 
@@ -127,8 +101,8 @@ Module Opal (NodeType VarType WorldVarType OpType: OrderedType).
   | AtCom : node -> com -> com
   | HandleCom : node -> var -> op -> sexp -> var -> var -> var -> sexp -> com -> com
   | OpCom : op -> com
-  | WorldAssignCom : worldvar -> world -> com
-  | CommitCom : world -> com
+  | WorldAssignCom : worldvar -> com -> com
+  | CommitCom : worldvar -> com
   with
   bool :=
   | TrueBool : bool
@@ -142,30 +116,49 @@ Module Opal (NodeType VarType WorldVarType OpType: OrderedType).
   | EmptySexp : sexp
   | ConsSexp : sexp -> sexp -> sexp
   | VarSexp : node -> var -> sexp
-  | WeightSexp : world -> node -> var -> sexp
-  with
-  world :=
-  | VarWorld : worldvar -> world
-  | HypWorld : com -> world
+  | WeightSexp : worldvar -> node -> var -> sexp
   .
 
-  Section Evaluation.
-    Definition sigma_t := NodeVarMap.t sexp.
-    Definition sigma_0 : sigma_t := NodeVarMap.empty sexp.
+  Inductive bool_value :=
+  | TrueBoolValue : bool_value
+  | FalseBoolValue : bool_value
+  .
+  Definition bool_of_bool_value (b: bool_value) : bool :=
+    match b with
+    | TrueBoolValue => TrueBool
+    | FalseBoolValue => FalseBool
+    end.
 
-    Definition sigma_get (sigma: sigma_t) (n: node) (v: var) : option sexp :=
+  Inductive sexp_value :=
+  | EmptySexpValue : sexp_value
+  | ConsSexpValue : sexp_value -> sexp_value -> sexp_value
+  .
+  Fixpoint sexp_of_sexp_value (s: sexp_value) : sexp :=
+    match s with
+    | EmptySexpValue => EmptySexp
+    | ConsSexpValue s1 s2 =>
+      ConsSexp (sexp_of_sexp_value s1)
+               (sexp_of_sexp_value s2)
+    end.
+
+
+  Section Evaluation.
+    Definition sigma_t := NodeVarMap.t sexp_value.
+    Definition sigma_0 : sigma_t := NodeVarMap.empty sexp_value.
+
+    Definition sigma_get (sigma: sigma_t) (n: node) (v: var) : option sexp_value :=
       NodeVarMap.find (n,v) sigma.
-    Definition sigma_set (sigma: sigma_t) (n: node) (v: var) (s: sexp) : sigma_t :=
+    Definition sigma_set (sigma: sigma_t) (n: node) (v: var) (s: sexp_value) : sigma_t :=
       NodeVarMap.add (n,v) s sigma.
 
-    Definition Sigma_t := list sigma_t.
-    Fixpoint Sigma_get (Sigma: Sigma_t) (n: node) (v: var) : option sexp :=
-      match Sigma with
+    Definition sigmas_t := list sigma_t.
+    Fixpoint sigmas_get (sigmas: sigmas_t) (n: node) (v: var) : option sexp_value :=
+      match sigmas with
       | nil => None
-      | (cons sigma Sigma) =>
+      | (cons sigma sigmas) =>
         match sigma_get sigma n v with
         | Some s => Some s
-        | None => Sigma_get Sigma n v
+        | None => sigmas_get sigmas n v
         end
       end.
 
@@ -177,6 +170,7 @@ Module Opal (NodeType VarType WorldVarType OpType: OrderedType).
       WorldVarMap.add u (sig_orig, sig_hyp) omega.
 
     Definition pi_t := NodeSet.t.
+    Definition pi_0 : pi_t := NodeSet.empty.
     Definition pi_add (n: node) (pi: pi_t) : pi_t :=
       NodeSet.add n pi.
     Definition pi_mem (n: node) (pi: pi_t) : Datatypes.bool :=
@@ -185,149 +179,164 @@ Module Opal (NodeType VarType WorldVarType OpType: OrderedType).
     Definition rho_t := node.
 
     Definition eta_t := OpMap.t (node * var * sexp).
+    Definition eta_0 : eta_t := OpMap.empty (node * var * sexp).
     Definition eta_get (eta: eta_t) (op: op) : option (node * var * sexp) :=
       OpMap.find op eta.
     Definition eta_set (eta: eta_t) (op: op) (n: node) (v: var) (sh: sexp) : eta_t :=
       OpMap.add op (n,v,sh) eta.
 
     Definition mu_t := NodeVarMap.t (var * var * var * sexp).
+    Definition mu_0 : mu_t := NodeVarMap.empty (var * var * var * sexp).
     Definition mu_get (mu: mu_t) (n: node) (v: var) : option (var * var * var * sexp) :=
       NodeVarMap.find (n,v) mu.
     Definition mu_set (mu: mu_t) (n: node) (v vo vh vc: var) (sm: sexp) : mu_t:=
       NodeVarMap.add(n,v) (vo,vh,vc,sm) mu.
 
-    Program Fixpoint eval_sexp (s: sexp) (Sigma: Sigma_t) (omega: omega_t) (pi: pi_t) (rho: rho_t) (eta: eta_t) (mu: mu_t) {s} : option sexp :=
+    Fixpoint eval_eq (l r: sexp_value) :=
+      match l, r with
+      | EmptySexpValue, EmptySexpValue => TrueBoolValue
+      | ConsSexpValue ll lr, ConsSexpValue rl rr =>
+        match eval_eq ll rl, eval_eq ll rl with
+        | TrueBoolValue, TrueBoolValue => TrueBoolValue
+        | _, _ => FalseBoolValue
+        end
+      | _, _ => FalseBoolValue
+      end.
+
+    Fixpoint eval_mem (l r: sexp_value) :=
+      match r with
+      | EmptySexpValue => FalseBoolValue
+      | ConsSexpValue rl rr =>
+        match eval_eq l rl, eval_mem l rr with
+        | TrueBoolValue, _ => TrueBoolValue
+        | _, TrueBoolValue => TrueBoolValue
+        | _, _ => FalseBoolValue
+        end
+      end.
+
+    Fixpoint eval_sexp (s: sexp) (sigmas: sigmas_t) (omega: omega_t) (pi: pi_t) : option sexp_value :=
       match s with
-      | EmptySexp => Some EmptySexp
+      | EmptySexp => Some EmptySexpValue
       | VarSexp n v =>
         if pi_mem n pi then
-          Sigma_get Sigma n v
+          sigmas_get sigmas n v
         else
           None
       | WeightSexp w n v =>
-        match eval_world w Sigma omega pi rho eta mu with
+        match omega_get omega w with
         | Some (sigma_orig, sigma_hyp) =>
-          sigma_get sigma_hyp n v
+          sigmas_get (cons sigma_hyp sigmas) n v
         | None =>
           None
         end
-    | ConsSexp s1 s2 =>
-      match eval_sexp s1 Sigma omega pi rho eta mu,
-            eval_sexp s2 Sigma omega pi rho eta mu with
-      | Some s1v, Some s2v =>
-        Some (ConsSexp s1v s2v)
-      | _, _ => None
-      end
-      end
-    with
-    eval_bool (b: bool) (Sigma: Sigma_t) (omega: omega_t) (pi: pi_t) (rho: rho_t) (eta: eta_t) (mu: mu_t) {b} : option bool :=
+      | ConsSexp s1 s2 =>
+        match eval_sexp s1 sigmas omega pi,
+              eval_sexp s2 sigmas omega pi with
+        | Some s1v, Some s2v =>
+          Some (ConsSexpValue s1v s2v)
+        | _, _ => None
+        end
+      end.
+
+    Fixpoint eval_bool (b: bool) (sigmas: sigmas_t) (omega: omega_t) (pi: pi_t) : option bool_value :=
       match b with
-      | TrueBool => Some TrueBool
-      | FalseBool => Some FalseBool
+      | TrueBool => Some TrueBoolValue
+      | FalseBool => Some FalseBoolValue
       | ConjBool b1 b2 =>
-        match eval_bool b1 Sigma omega pi rho eta mu,
-              eval_bool b2 Sigma omega pi rho eta mu
+        match eval_bool b1 sigmas omega pi,
+              eval_bool b2 sigmas omega pi
         with
-        | Some TrueBool, Some b2' => Some b2'
-        | Some FalseBool, Some b2' => Some FalseBool
+        | Some TrueBoolValue, Some b2' => Some b2'
+        | Some FalseBoolValue, Some b2' => Some FalseBoolValue
         | _, _ => None
         end
       | DisjBool b1 b2 =>
-        match eval_bool b1 Sigma omega pi rho eta mu,
-              eval_bool b2 Sigma omega pi rho eta mu
+        match eval_bool b1 sigmas omega pi,
+              eval_bool b2 sigmas omega pi
         with
-        | Some FalseBool, Some b2' => Some b2'
-        | Some TrueBool, Some b2' => Some TrueBool
+        | Some FalseBoolValue, Some b2' => Some b2'
+        | Some TrueBoolValue, Some b2' => Some TrueBoolValue
         | _, _ => None
         end
       | EqBool s1 s2 =>
-        match eval_sexp s1 Sigma omega pi rho eta mu,
-              eval_sexp s2 Sigma omega pi rho eta mu
+        match eval_sexp s1 sigmas omega pi,
+              eval_sexp s2 sigmas omega pi
         with
-        | Some EmptySexp, Some EmptySexp => Some TrueBool
-        | Some (ConsSexp s1l s1r), Some (ConsSexp s2l s2r) =>
-          eval_bool (ConjBool (EqBool s1l s2l) (EqBool s1r s2r)) Sigma omega pi rho eta mu
-        | Some EmptySexp, Some _ => Some FalseBool
-        | Some _, Some EmptySexp => Some FalseBool
+        | Some l, Some r => Some (eval_eq l r)
         | _, _ => None
         end
       | MemBool s1 s2 =>
-        match eval_sexp s1 Sigma omega pi rho eta mu,
-              eval_sexp s2 Sigma omega pi rho eta mu
+        match eval_sexp s1 sigmas omega pi,
+              eval_sexp s2 sigmas omega pi
         with
-        | Some _, Some EmptySexp => Some FalseBool
-        | Some s1', Some (ConsSexp s2l s2r) =>
-          eval_bool (DisjBool (EqBool s1' s2l) (MemBool s1' s2r)) Sigma omega pi rho eta mu
+        | Some l, Some r => Some (eval_mem l r)
         | _, _ => None
         end
-      end
-    with
-    eval_com (c: com) (Sigma: Sigma_t) (omega: omega_t) (pi: pi_t) (rho: rho_t) (eta: eta_t) (mu: mu_t) {c} : option (sigma_t * omega_t) :=
-      match Sigma with
+      end.
+
+    Fixpoint eval_com (c: com) (sigmas: sigmas_t) (omega: omega_t) (pi: pi_t) (rho: rho_t) (eta: eta_t) (mu: mu_t) : option (sigma_t * omega_t) :=
+      match sigmas with
       | nil => None
-      | cons sigma Simga =>
+      | cons sigma sigmas =>
         match c with
         | SkipCom => Some (sigma, omega)
         | SeqCom c1 c2 =>
-          match eval_com c1 (cons sigma Sigma) omega pi rho eta mu with
+          match eval_com c1 (cons sigma sigmas) omega pi rho eta mu with
           | None => None
           | Some (sigma', omega') =>
-            eval_com c2 (cons sigma' Sigma) omega' pi rho eta mu
+            eval_com c2 (cons sigma' sigmas) omega' pi rho eta mu
           end
         | IfCom b c1 c2 =>
-          match eval_bool b (cons sigma Sigma) omega pi rho eta mu with
-          | Some TrueBool =>
-            eval_com c1 (cons sigma Sigma) omega pi rho eta mu
-          | Some FalseBool =>
-            eval_com c2 (cons sigma Sigma) omega pi rho eta mu
+          match eval_bool b (cons sigma sigmas) omega pi with
+          | Some TrueBoolValue =>
+            eval_com c1 (cons sigma sigmas) omega pi rho eta mu
+          | Some FalseBoolValue =>
+            eval_com c2 (cons sigma sigmas) omega pi rho eta mu
           | _ => None
           end
         | WithCom n c =>
-          eval_com c (cons sigma Sigma) omega (pi_add n pi) rho eta mu
+          eval_com c (cons sigma sigmas) omega (pi_add n pi) rho eta mu
         | AtCom n c =>
-          eval_com c (cons sigma Sigma) omega pi n eta mu
+          eval_com c (cons sigma sigmas) omega pi n eta mu
         | HandleCom n v op sh vo vh vc sm c =>
           if pi_mem n pi then
-            eval_com c (cons sigma Sigma) omega pi n (eta_set eta op n v sh) (mu_set mu n v vo vh vc sm)
+            eval_com c (cons (sigma_set sigma n v EmptySexpValue) sigmas) omega pi n (eta_set eta op n v sh) (mu_set mu n v vo vh vc sm)
           else
             None
         | OpCom op =>
           match eta_get eta op with
           | Some (n, v, sh) =>
-            if pi_mem n pi then
-              match eval_sexp sh (cons sigma Sigma) omega pi rho eta mu with
-              | None => None
-              | Some s' =>
-                Some (sigma_set sigma n v s', omega)
-              end
-            else
-              None
+            match eval_sexp sh (cons sigma sigmas) omega pi with
+            | None => None
+            | Some s' =>
+              Some (sigma_set sigma n v s', omega)
+            end
           | None => None
           end
-        | WorldAssignCom u w =>
-          match eval_world w (cons sigma Sigma) omega pi rho eta mu with
+        | WorldAssignCom u c =>
+          match eval_com c (cons sigma_0 (cons sigma sigmas)) omega_0 pi rho eta mu with
           | None => None
-          | Some (sigma_orig, sigma_hyp) =>
-            Some (sigma, omega_set omega u sigma_orig sigma_hyp)
+          | Some (sigma_hyp, omega_hyp) =>
+            Some (sigma, omega_set omega u sigma sigma_hyp)
           end
         | CommitCom w =>
-          match eval_world w (cons sigma Sigma) omega pi rho eta mu with
+          match omega_get omega w with
           | None => None
           | Some (sigma_orig, sigma_hyp) =>
-            let merged_sigma : NodeVarMap.t (option sexp) :=
+            let merged_sigma : NodeVarMap.t (option sexp_value) :=
                 NodeVarMap.mapi
                   (fun key sh =>
-                     match key return option sexp with
+                     match key with
                      | (n, v) =>
                        match mu_get mu n v,
-                             Sigma_get (cons sigma Sigma) n v,
-                             Sigma_get (cons sigma_orig Sigma) n v
+                             sigmas_get (cons sigma sigmas) n v,
+                             sigmas_get (cons sigma_orig sigmas) n v
                        with
                        | Some (vo, vh, vc, sm), Some sc, Some so =>
                          let sigma_o := sigma_set sigma n vo so in
                          let sigma_oh := sigma_set sigma_o n vh sh in
                          let sigma_ohc := sigma_set sigma_oh n vc sc in
-                         eval_sexp sm (cons sigma_ohc Sigma) omega pi rho eta mu
+                         eval_sexp sm (cons sigma_ohc sigmas) omega pi
                        | _, _, _ => None
                        end
                      end)
@@ -348,27 +357,370 @@ Module Opal (NodeType VarType WorldVarType OpType: OrderedType).
             end
           end
         end
-      end
-    with
-    eval_world (w: world) (Sigma: Sigma_t) (omega: omega_t) (pi: pi_t) (rho: rho_t) (eta: eta_t) (mu: mu_t) : option (sigma_t * sigma_t) :=
-      match Sigma with
-      | nil => None
-      | cons sigma Sigma =>
-        match w with
-        | VarWorld u =>
-          omega_get omega u
-        | HypWorld c =>
-          match eval_com c (cons sigma_0 (cons sigma Sigma)) omega_0 pi rho eta mu with
-          | None => None
-          | Some (sigma_hyp, omega_hyp) =>
-            Some (sigma, sigma_hyp)
-          end
-        end
-      end
+      end.
+  End Evaluation.
+
+  Section WellFormed.
+    Definition Omega_t := WorldVarSet.t.
+    Definition Sigma_t := NodeVarSet.t.
+    Definition Pi_t := NodeSet.t.
+    Definition H_t := OpSet.t.
+
+    Inductive well_formed_sexp : sexp -> Omega_t -> Sigma_t -> Pi_t -> Prop :=
+    | EmptySexpWellFormed : forall Omega Sigma Pi,
+        well_formed_sexp EmptySexp Omega Sigma Pi
+    | ConsSexpWellFormed : forall l r Omega Sigma Pi,
+        well_formed_sexp l Omega Sigma Pi ->
+        well_formed_sexp r Omega Sigma Pi ->
+        well_formed_sexp (ConsSexp l r) Omega Sigma Pi
+    | VarSexpWellFormed : forall n v Omega Sigma Pi,
+        NodeVarSet.In (n,v) Sigma ->
+        NodeSet.In n Pi ->
+        well_formed_sexp (VarSexp n v) Omega Sigma Pi
+    | WeightSexpWellFormed : forall u n v Omega Sigma Pi,
+        WorldVarSet.In u Omega ->
+        NodeVarSet.In (n,v) Sigma ->
+        NodeSet.In n Pi ->
+        well_formed_sexp (WeightSexp u n v) Omega Sigma Pi
     .
 
-    Obligation Tactic := admit.
-    Solve All Obligations.
+    Inductive well_formed_bool : bool -> Omega_t -> Sigma_t -> Pi_t -> Prop :=
+    | TrueBoolWellFormed : forall Omega Sigma Pi,
+        well_formed_bool TrueBool Omega Sigma Pi
+    | FalseBoolWellFormed : forall Omega Sigma Pi,
+        well_formed_bool FalseBool Omega Sigma Pi
+    | ConjBoolWellFormed : forall l r Omega Sigma Pi,
+        well_formed_bool l Omega Sigma Pi ->
+        well_formed_bool r Omega Sigma Pi ->
+        well_formed_bool (ConjBool l r) Omega Sigma Pi
+    | DisjBoolWellFormed : forall l r Omega Sigma Pi,
+        well_formed_bool l Omega Sigma Pi ->
+        well_formed_bool r Omega Sigma Pi ->
+        well_formed_bool (DisjBool l r) Omega Sigma Pi
+    | EqSexpWellFormed : forall l r Omega Sigma Pi,
+        well_formed_sexp l Omega Sigma Pi ->
+        well_formed_sexp r Omega Sigma Pi ->
+        well_formed_bool (EqBool l r) Omega Sigma Pi
+    | MemSexpWellFormed : forall l r Omega Sigma Pi,
+        well_formed_sexp l Omega Sigma Pi ->
+        well_formed_sexp r Omega Sigma Pi ->
+        well_formed_bool (MemBool l r) Omega Sigma Pi
+    .
+
+    Inductive well_formed_com : com -> Omega_t -> Sigma_t -> Pi_t -> H_t -> Omega_t -> Prop :=
+    | SkipComWellFormed : forall Omega Sigma Pi H Omega',
+        well_formed_com SkipCom Omega Sigma Pi H Omega'
+    | SeqComWellFormed : forall l r Omega Sigma Pi H Omega' Omega'',
+        well_formed_com l Omega Sigma Pi H Omega' ->
+        well_formed_com r Omega' Sigma Pi H Omega'' ->
+        well_formed_com SkipCom Omega Sigma Pi H Omega''
+    | IfComWellFormed : forall b l r Omega Sigma Pi H Omega' Omega'',
+        well_formed_bool b Omega Sigma Pi ->
+        well_formed_com l Omega Sigma Pi H Omega' ->
+        well_formed_com r Omega Sigma Pi H Omega'' ->
+        well_formed_com (IfCom b l r) Omega Sigma Pi H
+                        (WorldVarSet.inter Omega' Omega'')
+    | WithComWellFormed : forall n c Omega Sigma Pi H Omega',
+        well_formed_com c Omega Sigma (NodeSet.add n Pi) H Omega' ->
+        well_formed_com (WithCom n c) Omega Sigma Pi H Omega'
+    | AtComWellFormed : forall n c Omega Sigma Pi H Omega',
+        well_formed_com c Omega Sigma Pi H Omega' ->
+        well_formed_com (AtCom n c) Omega Sigma Pi H Omega'
+    | WorldAssignComWellFormed : forall u c Omega Sigma Pi H Omega',
+        well_formed_com c WorldVarSet.empty Sigma Pi H Omega' ->
+        well_formed_com (WorldAssignCom u c) Omega Sigma Pi H (WorldVarSet.add u Omega)
+    | CommitComWellFormed : forall u Omega Sigma Pi H,
+        WorldVarSet.In u Omega ->
+        well_formed_com (CommitCom u) Omega Sigma Pi H (WorldVarSet.remove u Omega)
+    | HandleComWellFormed : forall n v op sh vo vh vc sm c Omega Sigma Pi H Omega',
+        NodeSet.In n Pi ->
+        NodeVarSet.In (n,v) Sigma ->
+        well_formed_sexp sh Omega (NodeVarSet.add (n,v) Sigma) Pi ->
+        well_formed_sexp sh Omega (NodeVarSet.add
+                                     (n,vc)
+                                     (NodeVarSet.add
+                                        (n,vh)
+                                        (NodeVarSet.add (n,vo) Sigma))) Pi ->
+        well_formed_com c Omega (NodeVarSet.add (n,v) Sigma) Pi (OpSet.add op H) Omega' ->
+        well_formed_com (HandleCom n v op sh vo vh vc sm c) Omega Sigma Pi H Omega'
+    | OpComWellFormed : forall op (Omega: Omega_t) Sigma Pi H Omega,
+        OpSet.In op H ->
+        well_formed_com (OpCom op) Omega Sigma Pi H Omega
+    .
+  End WellFormed.
+
+  Definition omega_reps (omega: omega_t) (Omega: Omega_t) :=
+    forall k, WorldVarSet.In k Omega -> WorldVarMap.In k omega.
+
+  Definition sigmas_reps (sigmas: sigmas_t) (Sigma: Sigma_t) : Prop :=
+    forall n v, NodeVarSet.In (n,v) Sigma ->
+                exists val, sigmas_get sigmas n v = Some val.
+
+  Definition eta_reps (eta: eta_t) (H: H_t) : Prop :=
+    forall op, OpSet.In op H ->
+                exists v, eta_get eta op = Some v.
+
+  Definition mu_reps (mu: mu_t) (Sigma: Sigma_t) : Prop :=
+    forall n v, NodeVarSet.In (n,v) Sigma ->
+                exists val, mu_get mu n v = Some val.
+
+  Theorem sexp_progress:
+    forall s omega sigma Omega Sigma Pi,
+      well_formed_sexp s Omega Sigma Pi ->
+      omega_reps omega Omega ->
+      sigmas_reps sigma Sigma ->
+      (exists sv, eval_sexp s sigma omega Pi = Some sv).
+  Proof.
+    induction s ; intros ; inversion H ; subst.
+    * unfold eval_sexp. eauto.
+    * specialize (IHs1 omega sigma Omega Sigma Pi).
+      specialize (IHs2 omega sigma Omega Sigma Pi).
+      intuition.
+      inversion H2. inversion H3.
+      unfold eval_sexp.
+      fold eval_sexp.
+      edestruct eval_sexp; edestruct eval_sexp; eauto.
+    * assert (pi_mem n Pi = true). specialize (NodeSet.mem_spec Pi n). crush.
+      unfold sigmas_reps in H1.
+      specialize (H1 n v H4).
+      inversion H1.
+      exists x.
+      unfold eval_sexp.
+      rewrite H2.
+      apply H3.
+    * assert (pi_mem n Pi = true). specialize (NodeSet.mem_spec Pi n). crush.
+      crush.
+      unfold omega_reps in H0.
+      specialize (H0 w).
+      intuition.
+      unfold omega_get.
+      inversion H3.
+      specialize (WorldVarMap.find_1 H0).
+      edestruct WorldVarMap.find ; intros ; try discriminate.
+      destruct p.
+      destruct (sigma_get s0 n v) ; eauto.
+  Qed.
+
+  Theorem bool_progress:
+    forall b omega sigma Omega Sigma Pi,
+      well_formed_bool b Omega Sigma Pi ->
+      omega_reps omega Omega ->
+      sigmas_reps sigma Sigma ->
+      (exists bv, eval_bool b sigma omega Pi = Some bv).
+  Proof.
+    induction b ; intros ; inversion H ; subst.
+    * unfold eval_bool. eauto.
+    * unfold eval_bool. eauto.
+    * specialize (IHb1 omega sigma Omega Sigma Pi H4 H0 H1).
+      specialize (IHb2 omega sigma Omega Sigma Pi H8 H0 H1).
+      crush.
+      destruct x0 ; eauto.
+    * specialize (IHb1 omega sigma Omega Sigma Pi H4 H0 H1).
+      specialize (IHb2 omega sigma Omega Sigma Pi H8 H0 H1).
+      crush.
+      destruct x0 ; eauto.
+    * specialize (sexp_progress) as sp1.
+      specialize (sexp_progress) as sp2.
+      specialize (sp1 s omega sigma Omega Sigma Pi H4 H0 H1).
+      specialize (sp2 s0 omega sigma Omega Sigma Pi H8 H0 H1).
+      crush.
+      eauto.
+    * specialize (sexp_progress) as sp1.
+      specialize (sexp_progress) as sp2.
+      specialize (sp1 s omega sigma Omega Sigma Pi H4 H0 H1).
+      specialize (sp2 s0 omega sigma Omega Sigma Pi H8 H0 H1).
+      crush.
+      eauto.
+  Qed.
 
 
+  Theorem progress:
+    forall c sigmas Sigma omega Omega Pi eta Eta mu rho,
+      sigmas <> nil ->
+      omega_reps omega Omega ->
+      sigmas_reps sigmas Sigma ->
+      eta_reps eta Eta ->
+      mu_reps mu Sigma ->
+      (exists Omega', well_formed_com c Omega Sigma Pi Eta Omega') ->
+      exists sigma' omega',
+        eval_com c sigmas omega Pi rho eta mu = Some (sigma', omega').
+  Proof.
+    induction c ; intros ; unfold eval_com ; fold eval_com.
+    * intros. destruct sigmas. contradiction H. reflexivity.
+      exists s. exists omega. auto.
+    * inversion H4.
+      inversion H5.
+    * inversion H4. inversion H5.
+      subst. intuition.
+
+      specialize (bool_progress).
+      intros.
+
+      destruct sigmas. contradiction H. reflexivity.
+      specialize (H6 b omega (s::sigmas) Omega Sigma Pi H10 H0 H1).
+      destruct (eval_bool b (s :: sigmas) omega Pi).
+      specialize (IHc1 (s::sigmas) Sigma omega Omega Pi eta Eta mu rho).
+      specialize (IHc2 (s::sigmas) Sigma omega Omega Pi eta Eta mu rho).
+      destruct b0.
+      - intuition.
+        eapply H9.
+        exists Omega'.
+        auto.
+      - intuition.
+        eapply H7.
+        exists Omega''.
+        auto.
+      - inversion H6. inversion H7.
+   * destruct sigmas. contradiction H. reflexivity.
+     specialize (IHc (s::sigmas) Sigma omega Omega (pi_add n Pi) eta Eta mu rho).
+     intuition.
+     assert (exists Omega' : Omega_t,
+                well_formed_com c Omega Sigma (pi_add n Pi) Eta Omega').
+      - inversion H4. inversion H6. subst. exists x. apply H15.
+      - crush.
+   * destruct sigmas. contradiction H. reflexivity.
+     specialize (IHc (s::sigmas) Sigma omega Omega Pi eta Eta mu n).
+     intuition.
+     assert (exists Omega' : Omega_t, well_formed_com c Omega Sigma Pi Eta Omega').
+      - destruct H4. exists x. inversion H4. auto.
+      - intuition.
+   * destruct sigmas. contradiction H. reflexivity.
+     inversion H4.
+     inversion H5.
+     assert (pi_mem n Pi = true). specialize (NodeSet.mem_spec Pi n). crush.
+     subst.
+     rewrite H26.
+     remember (sigma_set s1 n v EmptySexpValue) as s2.
+     pose (OpSet.add o Eta).
+     pose (NodeVarSet.add (n,v) Sigma).
+     specialize (IHc (s2::sigmas) (NodeVarSet.add (n, v) Sigma) omega Omega Pi (eta_set eta o n v s) t (mu_set mu n v v0 v1 v2 s0) n).
+     intuition.
+
+     assert (s2 :: sigmas = nil -> False).
+     intros. discriminate.
+
+     assert (sigmas_reps (s2 :: sigmas) (NodeVarSet.add (n, v) Sigma)).
+     unfold sigmas_reps in *.
+     unfold sigmas_get in *.
+     unfold sigma_set in *.
+     intros.
+     destruct (NodeVarType.eq_dec (n,v) (n0,v3)).
+      - specialize (NodeVarMap.add_1 s1 EmptySexpValue e).
+        intros.
+        exists (EmptySexpValue).
+        specialize (NodeVarMap.find_1 H8).
+        intros.
+        rewrite <- Heqs2 in H9.
+        assert (sigma_get s2 n0 v3 = Some EmptySexpValue).
+        + crush.
+        + rewrite H10. auto.
+      - fold sigmas_get in *.
+        specialize (H1 n0 v3).
+        specialize (NodeVarSet.add_spec Sigma (n,v) (n0,v3)).
+        intros.
+        destruct H8.
+        intuition.
+        destruct (sigma_get s2 n0 v3) eqn:?.
+        + exists s3. auto.
+        + inversion H10.
+          destruct (sigma_get s1 n0 v3) eqn:?.
+          ** subst.
+             unfold sigma_get in *.
+             specialize (NodeVarMap.find_2 Heqo1).
+             intros.
+             specialize (NodeVarMap.add_2 EmptySexpValue n1 H13).
+             intros.
+             specialize (NodeVarMap.find_1 H14).
+             intros.
+             assert (sigma_get (NodeVarMap.add (n, v) EmptySexpValue s1) n0 v3 = Some s3). unfold sigma_get. auto.
+             assert (sigma_get (NodeVarMap.add (n, v) EmptySexpValue s1) n0 v3 = None). unfold sigma_get. auto.
+             rewrite H16 in H17. discriminate.
+          ** auto.
+-
+     assert (eta_reps (eta_set eta o n v s) t).
+     unfold eta_reps in *.
+     intros.
+     unfold eta_get in *.
+     unfold eta_set in *.
+     destruct (OpType.eq_dec o op0).
+     specialize (OpMap.add_1 eta (n,v,s) e).
+     exists (n,v,s).
+     specialize (OpMap.find_1 H9).
+     intros.
+     auto.
+     subst.
+     specialize H2 with op0.
+     assert (OpSet.In op0 Eta).
+     specialize (OpSet.add_spec Eta o op0).
+     intuition.
+     intuition.
+     inversion H11.
+     exists x0.
+     specialize (OpMap.find_2 H2).
+     intros.
+     specialize (OpMap.add_2 (n,v,s) n0 H12).
+     intros.
+     specialize (OpMap.find_1 H13).
+     auto.
+
+     assert (mu_reps (mu_set mu n v v0 v1 v2 s0) (NodeVarSet.add (n, v) Sigma)).
+     unfold mu_reps in *.
+     unfold mu_get in *.
+     unfold mu_set in *.
+     intros.
+     destruct (NodeVarType.eq_dec (n,v) (n0,v3)) eqn:?.
+     + specialize (NodeVarMap.add_1 mu (v0, v1, v2, s0) e).
+       intros.
+       specialize (NodeVarMap.find_1 H10).
+       intros.
+       exists (v0,v1,v2,s0). auto.
+     + specialize (H3 n0 v3).
+       assert (NodeVarSet.In (n0, v3) Sigma).
+       specialize (NodeVarSet.add_spec Sigma (n,v) (n0,v3)).
+       intros.
+       destruct H10. intuition.
+       intuition.
+       inversion H11.
+       specialize (NodeVarMap.find_2 H3).
+       intros.
+       specialize (NodeVarMap.add_2 (v0, v1, v2, s0) n1 H13).
+       intros.
+       exists x0.
+       specialize (NodeVarMap.find_1 H14).
+       intros.
+       auto.
+     + assert (exists Omega', well_formed_com c Omega (NodeVarSet.add (n, v) Sigma) Pi t Omega').
+     exists x. auto.
+
+     intuition.
+   * destruct sigmas. contradiction H. reflexivity.
+     inversion H4.
+     inversion H5.
+     subst.
+     unfold eta_reps in *.
+     unfold eta_get in *.
+     specialize (H2 o H8).
+     inversion H2.
+     rewrite H6.
+     destruct x0, p.
+     pose
+
+    subst. intuition.
+    specialize (IHc n Pi).
+    eapply IHc.
+    eauto.
+  * inversion H. inversion H0.
+    subst. intuition.
+    specialize (IHc n Pi).
+    assert (pi_mem n Pi = true). inversion H16.
+    crush.
+      - inversion H16; subst.
+        +
+
+    specialize (NodeSet.mem_spec Pi n). crush.
+    assert
+    inversion H16.
+    crush.
+    eapply IHc.
+  Qed.
 End Opal.
